src/StandardLibrary/UInt.dfy
@@ -19,11 +19,11 @@ module StandardLibrary.UInt {
 
   predicate method UInt8Less(a: uint8, b: uint8) { a < b }
 
-  predicate method IsSeq16<T>(s: seq<T>) {
+  predicate method HasUint16Len<T>(s: seq<T>) {
     |s| < UINT16_LIMIT
   }
 
-  type seq16<T> = s: seq<T> | IsSeq16(s)
+  type seq16<T> = s: seq<T> | HasUint16Len(s)
   type Uint8Seq16 = seq16<uint8>
 
   function method UInt16ToSeq(x: uint16): (ret: seq<uint8>)
